fstar_out/Set.ml
@@ -1,40 +1,30 @@
 open Prims
-type ordering = Compare.ordering
-type 'a comparaison = 'a Compare.comparaison
-type ('a, 'compare) set = ('a, unit) BinTree.set
-let mem : 'a . 'a comparaison -> 'a -> ('a, unit) set -> Prims.bool =
+type ('a, 'f) set = ('a, unit, unit) BinTree.set
+let mem : 'a . 'a Compare.comparaison -> 'a -> ('a, unit) set -> Prims.bool =
   fun f -> fun x -> fun input -> AVL.mem f x input
-let add : 'a . 'a comparaison -> 'a -> ('a, unit) set -> ('a, unit) set =
-  fun f -> fun x -> fun input -> AVL.add f x input
-let remove : 'a . 'a comparaison -> 'a -> ('a, unit) set -> ('a, unit) set =
-  fun f -> fun x -> fun input -> AVL.remove f x input
-let find_min :
-  'a . 'a comparaison -> ('a, unit) set -> 'a FStar_Pervasives_Native.option
+let member :
+  'a . 'a Compare.comparaison -> 'a -> ('a, unit) set -> Prims.bool =
+  fun f ->
+    fun x ->
+      fun input ->
+        match AVL.find f x input with
+        | FStar_Pervasives_Native.Some (k, uu___) -> k = x
+        | FStar_Pervasives_Native.None -> false
+let find :
+  'a .
+    'a Compare.comparaison ->
+      'a -> ('a, unit) set -> 'a FStar_Pervasives_Native.option
   =
   fun f ->
-    fun input ->
-      match input with
-      | BinTree.Leaf -> FStar_Pervasives_Native.None
-      | BinTree.Node (l, k, uu___, r) ->
-          FStar_Pervasives_Native.Some (AVL.find_min f input)
-let find_max :
-  'a . 'a comparaison -> ('a, unit) set -> 'a FStar_Pervasives_Native.option
-  =
-  fun f ->
-    fun input ->
-      match input with
-      | BinTree.Leaf -> FStar_Pervasives_Native.None
-      | BinTree.Node (l, k, uu___, r) ->
-          FStar_Pervasives_Native.Some (AVL.find_max f input)
-let remove_min : 'a . 'a comparaison -> ('a, unit) set -> ('a, unit) set =
-  fun f ->
-    fun input ->
-      match input with
-      | BinTree.Leaf -> BinTree.Leaf
-      | BinTree.Node (l, k, uu___, r) -> AVL.remove_min f input
-let remove_max : 'a . 'a comparaison -> ('a, unit) set -> ('a, unit) set =
-  fun f ->
-    fun input ->
-      match input with
-      | BinTree.Leaf -> BinTree.Leaf
-      | BinTree.Node (l, k, uu___, r) -> AVL.remove_max f input
+    fun x ->
+      fun input ->
+        match AVL.find f x input with
+        | FStar_Pervasives_Native.Some (y, uu___) ->
+            FStar_Pervasives_Native.Some y
+        | FStar_Pervasives_Native.None -> FStar_Pervasives_Native.None
+let add :
+  'a . 'a Compare.comparaison -> ('a, unit) set -> 'a -> ('a, unit) set =
+  fun f -> fun s -> fun x -> AVL.add f (x, ()) s
+let remove :
+  'a . 'a Compare.comparaison -> ('a, unit) set -> 'a -> ('a, unit) set =
+  fun f -> fun s -> fun x -> AVL.remove f x s
