Set.fst
@@ -1,7 +1,47 @@
 module Set 
 
-module C  = Compare 
 module BT = BinTree
 
-open BinTree
+open Compare
+
+let set (a:eqtype) (f: comparaison a) = s:BT.set a unit f{BT.is_avl s}
+
+let mem (#a: eqtype) (#f: comparaison a) (x:a) (input: set a f) : out:bool{out <==> (
+        exists y. BT.member (y, ()) input /\ EQ? (f x y)
+    )} = AVL.mem_lemma x input; AVL.mem x input
+
+let member (#a: eqtype) (#f: comparaison a) (x:a) (input: set a f) : out:bool{
+        out <==> BT.member (x, ()) input
+    } = 
+    AVL.find_lemma x input;
+    AVL.lemma_EQ (x, ()) input;
+
+    match AVL.find x input with 
+    | Some (k, _) -> k = x
+    | None -> false
+
+let find (#a: eqtype) (#f: comparaison a) (x:a) (input: set a f) : out:option a {
+        match out with 
+        | None -> ~(mem x input)
+        | Some y -> member y input /\ EQ? (f x y)
+    } = 
+    AVL.find_lemma x input; 
+
+    match AVL.find x input with 
+    | Some (y, _) -> Some y
+    | None -> None
+
+
+let add (#a: eqtype) (#f: comparaison a) (s:set a f) (x:a) : (out:set a f {
+        forall y. member y out <==> (if EQ? (f x y) then x == y else  member y s)
+    }) = 
+    AVL.add_lemma (x, ()) s;
+    AVL.add (x, ()) s
+
+
+let remove (#a: eqtype) (#f: comparaison a) (s:set a f) (x:a) : (out:set a f {
+        forall y. member y out <==> (member y out /\ ~(EQ? (f x y)))
+    }) = 
+    AVL.remove_lemma x s; 
+    AVL.remove x s
 
